Lean/step.lean
@@ -1,0 +1,47 @@
+import library
+import tactic
+
+open rpp
+
+namespace rpp
+
+def step (f : rpp) :=
+  ⌊2, 0, 1⌉ ;;
+  If Su Id₁ Id₁ ;;
+  Sw ;;
+  If (Pr ‖ Su) (Id₁ ‖ f ;; Sw) Id₁ ;;
+  ⌊2, 0, 1⌉ ;;
+  If Pr Id₁ Id₁ ;;
+  Sw
+
+lemma step_succ (f : rpp) (x y : ℕ) (z : list ℤ) :
+  ‹step f› (0 :: x :: y.succ :: z) = 0 :: x.succ :: y :: z :=
+by simp [step, ev, rewire]
+
+lemma step_zero (f : rpp) (x : ℕ) (z : list ℤ) :
+  ‹step f› (0 :: x :: 0 :: z) = 0 :: 0 :: ‹f› (x :: z) :=
+begin
+  rcases h : ‹f› (↑x :: z),
+  { apply_fun list.length at h, simp * at * },
+  { simp [step, ev, rewire, *] }
+end
+
+def cp_in :=
+  inc ;;
+  Id₁ ‖ It (Su ;; inc) ;;
+  Id₁ ‖ dec ;;
+  dec ;;
+  ⌊0, 3, 1⌉ ;;
+  inc ;;
+  Id₁ ‖ Sw
+
+def cu_in := It (step Su)
+
+def cp :=
+  cp_in ;;
+  ⌊2, 3, 0, 1⌉ ;;
+  cu_in⁻¹
+
+def div := It (step (Id₁ ‖ Su))
+
+end rpp
